switch from hom to upi; some first steps

analysis.v
@@ -1,13 +1,13 @@
 Require Import Coq.Classes.EquivDec.
 Require Import Coq.Bool.Bool.
 Require Import Coq.Logic.Eqdep_dec.
+Require Import Coq.Program.Equality.
 Require Import List.
 Require Import Nat.
 Require Import Omega.
 Require Import Ensembles.
 
-Module CFG.
-  Parameter N : nat.
+Module Uniana.
   Parameter Lab : Type.
   Parameter Var : Type.
   Parameter Val : Type.
@@ -19,13 +19,13 @@ Module CFG.
   Definition Coord := prod Lab IVec.
   Definition Conf := prod Coord State.
 
-  Definition UniState := Var -> Prop.
+  Definition UniState := Var -> bool.
 
   Parameter eff : Conf -> option Conf.
   Parameter abs_uni_eff : UniState -> UniState.
 
   Definition uni_state_concr (uni : UniState) : State -> State -> Prop :=
-    fun s => fun s' => forall x, uni x -> s x = s' x.
+    fun s => fun s' => forall x, uni x = true -> s x = s' x.
 
   Parameter local_uni_corr : forall uni p i q j s s' qs qs', 
       uni_state_concr uni s s' ->
@@ -55,6 +55,17 @@ Module CFG.
   Parameter edge_spec :
     forall p q, is_effect_on p q -> has_edge p q = true.
 
+  Notation "p --> q" := (has_edge p q = true) (at level 70, right associativity).
+
+  Lemma edge_spec2 :
+    forall p q i j s r, eff (p, i, s) = Some (q, j, r) -> (p --> q).
+  Proof.
+    intros.
+    eapply edge_spec.
+    exists i; exists j; exists s; exists r.
+    assumption.
+  Qed.
+
   Parameter def_spec :
     forall p q x, (exists i j s r, eff (p, i, s) = Some (q, j, r) /\ r x <> s x) -> is_def x p q = true.
 
@@ -79,7 +90,7 @@ Module CFG.
 
   (* TODO *)
   Inductive Tr : Conf -> Type :=
-    | Init : forall s, Tr (start_coord, s)
+    | Init : forall s, Tr (root, start_ivec, s)
     | Step : forall k k', Tr k' -> eff k' = Some k -> Tr k.
 
   Ltac inv_tr H := inversion H; subst; 
@@ -100,11 +111,12 @@ Module CFG.
   Definition sem_hyper (T : Hyper) : Hyper :=
     fun ts' => exists ts, T ts /\ ts' = sem_trace ts.
 
-  Definition Uni := Lab -> Var -> Prop.
-  Definition Hom := Lab -> Prop.
+  Definition Uni := Lab -> Var -> bool.
+  Definition Hom := Lab -> bool.
   Definition Unch := Lab -> Var -> Lab.
+  Definition Upi := Lab -> Lab -> bool.
 
-  Inductive In : forall k, Tr k -> Conf -> Prop := (* (k : Conf) (tr : Tr k) : Conf -> Prop :=  *)
+  Inductive In : forall k, Tr k -> Conf -> Prop :=
     | In_At : forall k tr, In k tr k
     | In_Other : forall l k k' tr' step, In k' tr' l -> In k (Step k k' tr' step) l.
 
@@ -124,23 +136,61 @@ Module CFG.
                                              Precedes (p, i, s) (Step (p, i, s) k t step) (q, j, r) (p, i, s)
   | Prec_other : forall k' k t c c' step, Precedes k t c c' ->
                                           Precedes k' (Step k' k t step) c c'.
-
-  Parameter nesting_spec : forall q p,
-      q <<= p ->
+  Definition unique_preceding q p :=
       forall k k' t t' j j' i r r' s s',
       Precedes k t (q, j, r) (p, i, s) ->
       Precedes k' t' (q, j', r') (p, i, s') ->
-      j' = j /\ r = r'.
+      j' = j.
+
+
+  Parameter nesting_spec : forall q p,
+      q <<= p ->
+      unique_preceding q p.
+
+  Inductive Path : Lab -> Lab -> Prop :=
+    | PathInit : forall p, Path p p
+    | PathStep : forall from p to, Path from p -> Is_true (has_edge p to) -> Path from to.
+
+  Inductive PathIn : forall from to, Path from to -> Lab -> Prop :=
+  | PathInAt : forall from to a, PathIn from to a to
+  | PathInOther : forall from q a p to edge, PathIn from q a p -> PathIn from to (PathStep from q to a edge) p.
+
+  Definition DisjointPaths (f1 f2 conv : Lab) (a : Path f1 conv) (b : Path f2 conv) :=
+    forall p, PathIn f1 conv a p -> PathIn f2 conv b p -> p === conv.
+    
+  Definition lab_of (k : Conf) :=
+    match k with
+      ((p, i), s) => p
+    end.
+
+  Parameter splits : Lab -> list (Lab * Var).
+
+  Parameter branch : Lab -> option (Lab * Lab * Var).
+
+  Parameter val_true : Val -> bool.
+
+  Parameter branch_spec : forall b,
+      match branch b with
+        | Some (t, f, x) => forall i s k, eff (b, i, s) = Some k -> lab_of k = (if val_true (s x) then t else f)
+        | None => forall i i' s s' k k', eff (b, i, s) = Some k ->
+                                         eff (b, i', s') = Some k' ->
+                                         lab_of k = lab_of k'
+      end.
+
+  Parameter splits_spec : forall br p q conv x, List.In (br, x) (splits conv) <->
+                                                (branch br = Some (p, q, x) /\
+                                                 (exists a b, DisjointPaths p q conv a b)).
+                                                
 
   Definition uni_concr (u : Uni) : Hyper :=
     fun ts => forall t t' tr tr', ts t tr -> ts t' tr' ->
                                   forall x p i s s', In t tr ((p, i), s) ->
                                                      In t' tr' ((p, i), s') ->
-                                                     u p x -> s x = s' x.
+                                                     u p x = true -> s x = s' x.
 
   Definition hom_concr (h : Hom) : Hyper :=
     fun ts => forall t t' tr tr', ts t tr -> ts t' tr' ->
-                                  forall p, h p ->
+                                  forall p, h p = true ->
                                             forall q q' j j'
                                                    i s s'
                                                    s1 s2, Follows t tr ((p, i), s1) ((q, j), s) ->
@@ -149,33 +199,33 @@ Module CFG.
 
   
   Definition unch_concr (unch : Unch) : Traces :=
-    fun k => fun t => forall to i s x, unch to x <<= to /\
-                                       (In k t (to, i, s) ->
+    fun k => fun t => forall to i s x, (In k t (to, i, s) ->
                                        exists j r, Precedes k t (unch to x, j, r) (to, i, s) /\ r x = s x).
 
-  Definition unch_trans_local (unch : Unch) (q p : Lab) (x : Var) : Lab :=
-    if is_def x q p then p else if nesting_dec (unch q x) p then unch q x else p.
+  Definition upi_concr (upi : Upi) : Hyper :=
+    fun ts => forall k k' t t',
+        ts k t -> ts k' t' ->
+        forall q p, upi q p = true ->
+                    forall j j' i r r' s s', Precedes k t (q, j, r) (p, i, s) ->
+                                             Precedes k' t' (q, j', r') (p, i, s') ->
+                                             j' = j.
 
-  Lemma unch_trans_local_nesting : forall unch q p x, unch_trans_local unch q p x <<= p.
-  Proof.
-    intros.
-    unfold unch_trans_local.
-    destruct (is_def x q p).
-    * apply nesting_refl.
-    * destruct (nesting_dec (unch q x) p).
-      - assumption.
-      - apply nesting_refl.
-  Qed.
+  Parameter upi_trans : Upi -> Uni -> Upi.
 
-  Lemma unch_trans_local_res : forall unch q p x, unch_trans_local unch q p x = p \/
-                                                  unch q x =/= p /\
-                                                  is_def x q p = false /\
-                                                  unch_trans_local unch q p x = unch q x.
+  Parameter upi_correct : forall upi uni t, sem_hyper (upi_concr upi) t -> upi_concr (upi_trans upi uni) t.
+
+  Definition unch_trans_local (upi : Upi) (uni: Uni) (unch : Unch) (q p : Lab) (x : Var) : Lab :=
+    if is_def x q p then p else if upi_trans upi uni (unch q x) p then unch q x else p.
+
+  Lemma unch_trans_local_res : forall upi uni unch q p x, unch_trans_local upi uni unch q p x = p \/
+                                                          unch q x =/= p /\
+                                                          is_def x q p = false /\
+                                                          unch_trans_local upi uni unch q p x = unch q x.
   Proof.
     intros.
     unfold unch_trans_local.
     destruct (is_def x q p); auto.
-    destruct (nesting_dec (unch q x) p); auto.
+    destruct (upi_trans upi uni (unch q x) p); auto.
     destruct (unch q x == p); auto.
   Qed.
 
@@ -189,26 +239,34 @@ Module CFG.
     | a :: l' => fold_right (fun a acc => if a == acc then a else default) a l'
     end.
 
-  Definition unch_trans (unch : Unch) : Unch :=
-    fun p => fun x => all_equal (map (fun q => unch_trans_local unch q p x) (preds p)) p.
+  Definition unch_trans (upi : Upi) (uni : Uni) (unch : Unch) : Unch :=
+    fun p => fun x => all_equal (map (fun q => unch_trans_local upi uni unch q p x) (preds p)) p.
 
-  Lemma unch_trans_nesting unch p x : unch_trans unch p x <<= p.
+  (*
+  Lemma unch_trans_res2 :
+    forall upi uni unch p x,
+      unch_trans upi uni unch p x = p \/ exists q, upi (unch q x) p = true.
   Proof.
     intros.
     unfold unch_trans.
-    destruct (preds p); simpl.
-    - apply nesting_refl.
-    - destruct l0; simpl.
-      + apply unch_trans_local_nesting.
-      + destruct ((unch_trans_local unch l0 p x) == _).
-        * apply unch_trans_local_nesting.
-        * apply nesting_refl.
-  Qed.      
+    destruct (preds p); intros; [ auto | simpl ].
+    induction l0; simpl in *.
+    - unfold unch_trans_local.
+      destruct (is_def x l p); auto.
+      remember (upi (unch l x) p) as upt.
+      symmetry in Hequpt.
+      destruct upt; auto.
+      right. exists l. assumption.
+    - destruct IHl0; try destruct (equiv_dec (unch_trans_local upi uni unch a p x) _); auto.
+      rewrite e. rewrite H. auto.
+  Qed.
+*)
 
-  Lemma unch_trans_res : forall unch q p x, is_effect_on q p ->
-                                            (unch_trans unch p x = p \/
-                                             unch q x =/= p /\ is_def x q p = false /\
-                                             unch_trans unch p x = unch q x).
+  Lemma unch_trans_res : forall upi uni unch q p x, q --> p ->
+                                                    (unch_trans upi uni unch p x = p \/
+                                                     unch q x =/= p /\ is_def x q p = false /\
+                                                     unch_trans_local upi uni unch q p x = unch q x /\
+                                                     unch_trans upi uni unch p x = unch q x).
   Proof.
     intros.
     unfold unch_trans.
@@ -216,24 +274,50 @@ Module CFG.
     - destruct (preds p); intros; [ auto | simpl ]. 
       induction l0; simpl in *.
       + inversion_clear H0; [ subst | contradiction ].
-        apply unch_trans_local_res.
+        assert (Hlocal := unch_trans_local_res upi uni unch q p x).
+        firstorder.
       + inversion_clear H0; subst; simpl.
-        * destruct ((unch_trans_local unch a p x) == _); auto.
+        * destruct ((unch_trans_local upi uni unch a p x) == _); auto.
           rewrite e.
           eapply IHl0.
           auto.
         * inversion_clear H1; subst; simpl.
-          -- destruct ((unch_trans_local unch q p x) == _); auto.
-             apply unch_trans_local_res.
-          -- destruct ((unch_trans_local unch a p x) == _); auto.
+          -- destruct ((unch_trans_local upi uni unch q p x) == _); auto.
+             assert (Hlocal := unch_trans_local_res upi uni unch q p x).
+             firstorder.
+          -- destruct ((unch_trans_local upi uni unch a p x) == _); auto.
              rewrite e.
              eapply IHl0.
              auto.
     - apply preds_spec.
-      apply edge_spec.
       assumption.
   Qed.
 
+  Lemma upi_unch :
+    forall upi uni unch p x,
+    unch_trans upi uni unch p x =/= p -> upi_trans upi uni (unch_trans upi uni unch p x) p = true .
+  Proof.
+    intros.
+    remember (preds p) as pr.
+    destruct pr.
+    + unfold unch_trans in H.
+      rewrite <- Heqpr in H.
+      simpl in H.
+      contradiction H; reflexivity.
+    + cut (List.In l (preds p)). intro Hedge.
+      - apply preds_spec in Hedge.
+        assert (Hunch := unch_trans_res upi uni unch l p x Hedge).
+        destruct Hunch as [Hunch | Hunch]; [ exfalso; contradiction H; reflexivity | ].
+        destruct Hunch as [Huneq [Hdef [Hlocal Hunch]]].
+        rewrite Hunch.
+        unfold unch_trans_local in Hlocal.
+        destruct (is_def x l p); [ inversion Hdef | clear Hdef ].
+        destruct (upi_trans upi uni (unch l x) p).
+        * reflexivity.
+        * exfalso; apply Huneq; symmetry; assumption.
+      - rewrite <- Heqpr. simpl. auto.
+  Qed.
+  
   Lemma list_emp_in : forall {A: Type} l, (forall (a: A), ~ List.In a l) -> l = nil.
   Proof.
     intros.
@@ -248,7 +332,7 @@ Module CFG.
         simpl in H. auto.
   Qed.
 
-  Lemma unch_trans_root : forall unch x, unch_trans unch root x = root.
+  Lemma unch_trans_root : forall upi uni unch x, unch_trans upi uni unch root x = root.
   Proof.
     intros.
     cut (preds root = nil); intros.
@@ -265,23 +349,57 @@ Module CFG.
         inversion H.
   Qed.
 
-  Parameter hom_trans : Hom -> Hom.
+  (*
+  Lemma trace_exists_path :
+    forall k tr p i s, In k tr (p, i, s) -> Path root p.
+  Proof.
+    intros k tr.
+    induction tr; intros; inv_tr H; [ constructor | | eauto ].
+    destruct k' as [[q j] r].
+    specialize (IHtr q j r).
+    eapply PathStep.
+    eapply IHtr.
+    constructor.
+    eapply edge_spec2; eapply e.
+  Qed.
+  *)
 
-  Parameter hom_trans_sound : forall hom t,
-      sem_hyper (hom_concr hom) t -> hom_concr (hom_trans hom) t.
-  
-  Definition uni_trans (uni : Uni) (hom : Hom) (unch : Unch) : Uni :=
+  Definition joinb (l : list bool) := fold_right andb true l.
+
+  Lemma joinb_true_iff {A : Type} : 
+    forall f (l : list A), (joinb (map f l) = true) -> (forall x, List.In x l -> f x = true).
+  Proof.
+    intros.
+    unfold joinb in H.
+    induction l; inversion H0; simpl in H; apply andb_true_iff in H; try subst; destruct H; auto.
+  Qed.
+
+  Definition uni_trans (uni : Uni) (upi : Upi) (unch : Unch) : Uni :=
     fun p => if p == root then uni root
-             else fun x => (hom_trans hom p /\ forall q, has_edge q p = true ->
-                                                         abs_uni_eff (uni q) x)
-                           \/ (let u := unch_trans unch p x in u =/= p /\ uni u x).
+             else fun x => ((joinb (map (fun spl => match spl with (s, x) => uni s x end) (splits p))) 
+                              && (joinb (map (fun q => abs_uni_eff (uni q) x) (preds p)))
+                              && (joinb (map (fun q => upi_trans upi uni q p) (preds p)))
+                           )
+                           || (let u := unch_trans upi uni unch p x in (u <>b p) && uni u x).
+
+  (*
+  Lemma x :
+    forall p i s s' q q' j r r' t t' eff eff' uni,
+                 Follows (p, i, s) (Step (p, i, s) (q, j, r) t eff) (p, i, s) (q, j, r) ->
+                 Follows (p, i, s') (Step (p, i, s') (q', j, r') t' eff') (p, i, s') (q', j, r') ->
+                 (forall sp x, List.In (sp, x) (splits p) -> uni sp x) ->
+                 q = q'.
+  Proof.
+  Qed.
+  *)
+
+    
 
   Lemma uni_trans_root_inv :
     forall uni hom unch x, uni_trans uni hom unch root x = uni root x.
   Proof.
     intros.
     unfold uni_trans.
-    simpl.
     destruct (equiv_dec root root).
     reflexivity.
     exfalso. apply c. reflexivity.
@@ -403,11 +521,6 @@ Module CFG.
     induction t; intros; inv_tr H; constructor; eauto.
    Qed.
 
-  Definition lab_of (k : Conf) :=
-    match k with
-      ((p, i), s) => p
-    end.
-
   Lemma follows_pred_unique :
     forall k' k t step d, Follows k' (Step k' k t step) k' d -> d = k.
   Proof.
@@ -419,7 +532,20 @@ Module CFG.
       eapply ivec_fresh in step1; [| apply H5].
       exfalso. auto.
   Qed.
-    
+
+  Lemma follows_implies_precedes :
+    forall k t p q i j s r,
+      p =/= q -> Follows k t (p, i, s) (q, j, r) -> Precedes k t (q, j, r) (p, i, s).
+  Proof.
+    intros k t p q i j s r Hneq Hflw.
+    induction t; inv_tr Hflw.
+    * constructor.
+      constructor.
+      assumption.
+    * econstructor.
+      auto.
+  Qed.
+
   Lemma precedes_follows :
     forall k t c d e,
       Precedes k t c d ->
@@ -490,15 +616,14 @@ Module CFG.
   Qed.
 
   Lemma unch_correct :
-    forall unch k t,
-      sem_trace (unch_concr unch) k t -> unch_concr (unch_trans unch) k t.
+    forall upi uni unch k t,
+      sem_trace (unch_concr unch) k t -> unch_concr (unch_trans upi uni unch) k t.
   Proof.
-    intros unch k t Hred.
+    intros upi uni unch k t Hred.
     unfold sem_trace in Hred.
     destruct Hred as [k' [t' [step [Hconcr H]]]]; subst.
     unfold unch_concr in *.
     intros to i s x.
-    split; [ apply unch_trans_nesting |].
     intros Hin.
     destruct (to == root).
     - rewrite e in *.
@@ -510,13 +635,13 @@ Module CFG.
     - apply follows_exists_detail in Hin; auto.
       destruct Hin as [q [j [r Hflw]]].
       specialize (Hconcr q j r x).
-      destruct Hconcr as [Hnest Hconcr].
       assert (Hinq := Hflw).
       apply follows_implies_in2_step in Hinq.
       specialize (Hconcr Hinq).
       destruct Hconcr as [h [u [Hprec Heq]]].
-      assert (Htrans := unch_trans_res unch q to x).
+      assert (Htrans := unch_trans_res upi uni unch q to x).
       destruct Htrans.
+      apply edge_spec.
       unfold is_effect_on.
       exists j. exists i. exists r. exists s.
       eapply follows_implies_step; eassumption.
@@ -525,7 +650,7 @@ Module CFG.
         split; [| reflexivity].
         apply precedes_self.
         eapply follows_implies_in; eassumption.
-      * destruct H as [Hqto [Hdef H]].
+      * destruct H as [Hqto [Hdef [_ H]]].
         rewrite H.
         exists h. exists u.
         split.
@@ -544,32 +669,32 @@ Module CFG.
     fun ts => h ts /\ h' ts.
 
   Lemma uni_correct :
-    forall uni hom unch t,
-        sem_hyper (red_prod (red_prod (uni_concr uni) (hom_concr hom)) (lift (unch_concr unch))) t ->
-        uni_concr (uni_trans uni hom unch) t.
+    forall uni upi unch t,
+        sem_hyper (red_prod (red_prod (uni_concr uni) (upi_concr upi)) (lift (unch_concr unch))) t ->
+        uni_concr (uni_trans uni upi unch) t.
   Proof.
-    intros uni hom unch t Hred.
+    intros uni upi unch t Hred.
     unfold sem_hyper in Hred.
     destruct Hred as [ts [Hconcr Hstep]].
     intros k k' tr tr' Hsem Hsem' x p i s s'.
     intros HIn HIn' Htrans.
 
-    assert (hom_concr (hom_trans hom) t) as HChom.
-    apply hom_trans_sound.
+    assert (upi_concr (upi_trans upi uni) t) as HCupi.
+    apply upi_correct.
     destruct Hconcr as [[_ Hhom] _].
     exists ts; auto.
 
-    assert (unch_concr (unch_trans unch) k tr) as HCunch.
+    assert (unch_concr (unch_trans upi uni unch) k tr) as HCunch.
     destruct Hconcr as [[_ _] Hunch].
     unfold lift in *; subst.
     apply unch_correct. assumption.
     
-    assert (unch_concr (unch_trans unch) k' tr') as HCunch'.
+    assert (unch_concr (unch_trans upi uni unch) k' tr') as HCunch'.
     destruct Hconcr as [[_ _] Hunch].
     unfold lift in *; subst.
     apply unch_correct. assumption.
 
-    destruct Hconcr as [[HCuni _] _].
+    destruct Hconcr as [[HCuni HCupi'] _].
 
     subst.
     destruct Hsem as [l [ltr [lstep [Hts Hlstep]]]]; subst.
@@ -583,39 +708,70 @@ Module CFG.
       - inv_tr HIn'.
         * exfalso. eapply start_no_tgt. eassumption.
         * eapply (HCuni l l' ltr ltr'); try eassumption.
-    + destruct Htrans as [[Hhom Hpred] | Hunch].
+
+    + rewrite orb_true_iff in Htrans.
+      destruct Htrans as [Htrans | Hunch].
         (* The uni/hom case *)
-      - apply follows_exists in HIn; try eassumption.
+      - repeat rewrite andb_true_iff in Htrans.
+        destruct Htrans as [[Hsplit Hpred] Hupi].
+        apply follows_exists in HIn; try eassumption.
         apply follows_exists in HIn'; try eassumption.
         destruct HIn as [[[q j] sq] Hflw].
         destruct HIn' as [[[q' j'] sq'] Hflw'].
-        cut (q = q' /\ j = j'); intros.
-        * inversion_clear H as [Hq Hj]; subst j' q'.
-          eapply (local_uni_corr (uni q) q j p i sq sq' s s'); unfold uni_state_concr in *.
-          ** intros.
-             unfold uni_concr in HCuni .
-             eapply (HCuni l l' ltr ltr' Hts Hts' x0 q j);
-               try eapply follows_implies_in2_step; eassumption.
-          ** eapply follows_implies_step; eassumption.
-          ** eapply follows_implies_step; eassumption.
-          ** apply Hpred.
-             eapply edge_spec.
-             unfold is_effect_on.
-             exists j. exists i. exists sq. exists s. eapply follows_implies_step. apply Hflw.
-        * eapply (HChom k k' _ _); try eassumption.
-          exists l; exists ltr; exists lstep; auto.
-          exists l'; exists ltr'; exists lstep'; auto.
+        assert (List.In q (preds p)) as Hqpred.
+        eapply preds_spec. eapply edge_spec. 
+        exists j. exists i. exists sq. exists s. eapply follows_implies_step. apply Hflw.
+        cut (q' = q); intros; subst.
+        * cut (j' = j); intros; subst.
+          -- eapply (local_uni_corr (uni q) q j p i sq sq' s s');
+               unfold uni_state_concr in *.
+             ** intros.
+                unfold uni_concr in HCuni .
+                eapply (HCuni l l' ltr ltr' Hts Hts' x0 q j);
+                  try eapply follows_implies_in2_step; eassumption.
+             ** eapply follows_implies_step; eassumption.
+             ** eapply follows_implies_step; eassumption.
+             ** eapply joinb_true_iff in Hpred.
+                eapply Hpred.
+                assumption.
+          -- (* unique preceding instances *)
+             destruct (p == q).
+             ** rewrite <- e in *; clear e.
+                admit.
+             ** eapply HCupi.
+                exists l; exists ltr; exists lstep; auto.
+                exists l'; exists ltr'; exists lstep'; auto.
+                eapply joinb_true_iff in Hupi.
+                eapply Hupi.
+                eassumption.
+                eapply follows_implies_precedes; try eassumption.
+                eapply follows_implies_precedes; try eassumption.
+        * (* disjoint paths! *)
+          admit.
+
         (* The unch case *)
       - specialize (HCunch p i s x).
         specialize (HCunch' p i s' x).
-        destruct HCunch as [Hnest [j [r [Hprec Heq]]]]; try eassumption.
-        destruct HCunch' as [_ [j' [r' [Hprec' Heq']]]]; try eassumption.
+        destruct HCunch as [j [r [Hprec Heq]]]; try eassumption.
+        destruct HCunch' as [j' [r' [Hprec' Heq']]]; try eassumption.
+        apply andb_true_iff in Hunch.
         destruct Hunch as [ Hlab Hunch ].
+        unfold nequiv_decb in Hlab.
+        unfold equiv_decb in Hlab.
+        apply negb_true_iff in Hlab.
+        destruct (equiv_dec (unch_trans upi uni unch p x));
+          [inversion Hlab | clear Hlab].
         rewrite <- Heq. rewrite <- Heq'.
-        cut (j = j'); intros.
+        cut (j' = j); intros.
         * subst j'.
-          eapply HCuni; [ apply Hts | apply Hts' | | | apply Hunch ].
+          eapply HCuni; [ apply Hts | apply Hts' | | | ].
           eapply precedes_step; eassumption.
           eapply precedes_step; eassumption.
-        * eapply nesting_spec; eassumption.
+          assumption.
+        * eapply HCupi.
+          -- exists l; exists ltr; exists lstep; auto.
+          -- exists l'; exists ltr'; exists lstep'; auto.
+          -- eapply upi_unch. apply c0.
+          -- eassumption.
+          -- eassumption.
 Qed.
